fix a mistake of the memory oracle

model/agp32RelationScript.sml
@@ -294,10 +294,14 @@ Definition Rel_def:
   (I (3,t) <> NONE ==> reg_data_vaild 3 s ==> (s.EX.EX_jump_sel ==> s.IF.IF_PC_input = (FUNPOW Next (THE (I (3,t))) a).PC)) /\                 
   (I (1,t) <> NONE ==> (~s.EX.EX_jump_sel ==> s.IF.IF_PC_input = (FUNPOW Next (THE (I (1,t)) - 1) a).PC + 4w)) /\
   (I (4,t) <> NONE ==> fext.ready ==> fext.mem = (FUNPOW Next (THE (I (4,t))) a).MEM) /\
+  (I (4,t) = NONE ==> I (3,t) <> NONE ==> fext.ready ==> fext.mem = (FUNPOW Next (THE (I (3,t)) - 1) a).MEM) /\
+  (I (4,t) = NONE ==> I (3,t) = NONE ==> I (2,t) <> NONE ==> fext.ready ==> fext.mem = (FUNPOW Next (THE (I (2,t)) - 1) a).MEM) /\
+  (I (4,t) = NONE ==> I (3,t) = NONE ==> I (2,t) = NONE ==> I (1,t) <> NONE ==> fext.ready ==> 
+   fext.mem = (FUNPOW Next (THE (I (1,t)) - 1) a).MEM) /\
   (~fext.ready ==> ~enable_stg 1 s) /\
   (~fext.ready ==> ~enable_stg 2 s) /\                                     
-  (I (5,t) <> NONE ==> s.data_out = (FUNPOW Next (THE (I (5,t))) a).data_out) /\
-  (I (5,t) <> NONE ==> reg_data_vaild 5 s ==> (s.R = (FUNPOW Next (THE (I (5,t))) a).R)) /\
+  (I (5,t-1) <> NONE ==> s.data_out = (FUNPOW Next (THE (I (5,t-1))) a).data_out) /\
+  (I (5,t-1) <> NONE ==> reg_data_vaild 5 si ==> (s.R = (FUNPOW Next (THE (I (5,t-1))) a).R)) /\
   (I (1,t) <> NONE ==> IF_PC_Rel s a (THE (I (1,t)))) /\
   (I (1,t) <> NONE ==> fext.ready ==> IF_instr_Rel s a (THE (I (1,t)))) /\
   (I (2,t) <> NONE ==> enable_stg 2 si ==> ID_Rel s a (THE (I (2,t)))) /\
